Add Booleans, almost all Naturals

03-untyped/03Untyped/Basic.lean
@@ -1,5 +1,6 @@
 import Mathlib.Tactic.Basic
 
+namespace Untyped
 
 namespace Section3
 
@@ -46,7 +47,6 @@ theorem induction_size (P : Lang → Prop) :
     intro ind s
     exact induction_size_specified P (size s + 1) ind s (by simp)
 
-
 lemma induction_depth_specified (P : Lang → Prop) :
   ∀ gen_sz, (∀ (s : Lang), (∀ r, depth r < depth s → P r) → P s) →
   ∀ s, depth s < gen_sz  → P s := by
@@ -66,3 +66,230 @@ theorem induction_depth (P : Lang → Prop) :
 #check Lang.recOn
 
 end Section3
+
+namespace Booleans
+
+inductive Term : Type
+| True : Term
+| False : Term
+| If (c t e : Term) : Term
+
+inductive Value : Term → Prop
+| TrueV : Value Term.True
+| FalseV : Value Term.False
+
+inductive Step : Term → Term → Prop
+| IfTrue : Step (Term.If Term.True t e) t
+| IfFalse : Step (Term.If Term.False t e) e
+| IfStep : Step c c' → Step (Term.If c t e) (Term.If c' t e)
+
+theorem determinism : Step t t₁ → Step t t₂ → t₁ = t₂ := by
+  intro s1 s2
+  induction s1 generalizing t₂ <;> cases s2
+  all_goals (
+    try contradiction
+    try grind
+  )
+
+def Normal : Term → Prop
+| t => ¬ ∃ t', Step t t'
+
+theorem value_is_normal : Value v → Normal v := by
+  intro hv
+  cases hv <;> intro ⟨ t', hstep ⟩ <;> cases hstep
+
+theorem normal_is_value : Normal v → Value v := by
+  intro hn
+  induction v <;> repeat constructor
+  rename_i c t e c_ih t_ih e_ih
+  cases c
+  · cases hn ⟨ _, Step.IfTrue ⟩
+  · cases hn ⟨ _, Step.IfFalse ⟩
+  · cases c_ih (by
+      intro ⟨ c', hstep ⟩
+      apply hn
+      exact ⟨ _, Step.IfStep hstep ⟩
+    )
+
+inductive MultiStep : Term → Term → Prop
+| Refl : MultiStep t t
+| Step : Step t t' → MultiStep t' t'' → MultiStep t t''
+
+lemma multi_step_multi_step : MultiStep t t' → MultiStep t' t'' → MultiStep t t'' := by
+  intro ms1 ms2
+  induction ms1
+  · assumption
+  · rename_i ih
+    apply MultiStep.Step
+    · assumption
+    · apply ih
+      assumption
+
+lemma multi_if_step : MultiStep c c' →
+  MultiStep (Term.If c t e) (Term.If c' t e) := by
+  intro ms
+  induction ms
+  · apply MultiStep.Refl
+  · apply MultiStep.Step
+    · apply Step.IfStep
+      assumption
+    · assumption
+
+theorem unique_normal_form :
+  MultiStep t v₁ → MultiStep t v₂ → Normal v₁ → Normal v₂ → v₁ = v₂ := by
+  intro ms1 ms2 hn1 hn2
+  induction ms1 generalizing v₂ <;> cases ms2
+  · rfl
+  · cases hn1 ⟨ _, by assumption ⟩
+  · cases hn2 ⟨ _, by assumption ⟩
+  · rename_i s2 _ ih t' s1 _
+    apply ih
+    · rw [determinism s2 s1]
+      assumption
+    · assumption
+    · assumption
+
+theorem termination : ∀ t, ∃ v, MultiStep t v ∧ Normal v := by
+  intro t
+  induction t
+  · exists Term.True
+    repeat constructor
+    apply value_is_normal
+    constructor
+  · exists Term.False
+    repeat constructor
+    apply value_is_normal
+    constructor
+  · rename_i c t e ihc iht ihe
+    have ⟨ vc, hc, hnc ⟩ := ihc
+    have ⟨ vt, ht, hnt ⟩ := iht
+    have ⟨ ve, he, hne ⟩ := ihe
+    cases normal_is_value hnc
+    · exists vt
+      constructor
+      · apply multi_step_multi_step
+        · apply multi_if_step hc
+        · apply MultiStep.Step
+          · exact Step.IfTrue
+          · assumption
+      · assumption
+    · exists ve
+      constructor
+      · apply multi_step_multi_step
+        · apply multi_if_step hc
+        · apply MultiStep.Step
+          · exact Step.IfFalse
+          · assumption
+      · assumption
+
+end Booleans
+
+namespace Naturals
+
+inductive Term : Type
+| True : Term
+| False : Term
+| If (c t e : Term) : Term
+| Zero : Term
+| Succ (t : Term) : Term
+| Pred (t : Term) : Term
+| IsZero (t : Term) : Term
+
+inductive NatV : Term → Prop
+| ZeroV : NatV Term.Zero
+| SuccV : NatV t → NatV (Term.Succ t)
+
+inductive Value : Term → Prop
+| TrueV : Value Term.True
+| FalseV : Value Term.False
+| NatV : NatV t → Value t
+
+inductive Step : Term → Term → Prop
+| IfTrue : Step (Term.If Term.True t e) t
+| IfFalse : Step (Term.If Term.False t e) e
+| IfStep : Step c c' → Step (Term.If c t e) (Term.If c' t e)
+| SuccStep : Step t t' → Step (Term.Succ t) (Term.Succ t')
+| PredZero : Step (Term.Pred Term.Zero) Term.Zero
+| PredSucc : NatV t → Step (Term.Pred (Term.Succ t)) t
+| PredStep : Step t t' → Step (Term.Pred t) (Term.Pred t')
+| IsZeroZero : Step (Term.IsZero Term.Zero) Term.True
+| IsZeroSucc : NatV t → Step (Term.IsZero (Term.Succ t)) Term.False
+| IsZeroStep : Step t t' → Step (Term.IsZero t) (Term.IsZero t')
+
+inductive MultiStep : Term → Term → Prop
+| Refl : MultiStep t t
+| Step : Step t t' → MultiStep t' t'' → MultiStep t t''
+
+lemma nv_no_step : NatV t → ¬ Step t t' := by
+  induction t generalizing t'
+  all_goals (
+    intro hnv
+    cases hnv
+    try contradiction
+  )
+  · intro s
+    cases s
+  · intro s
+    cases s
+    grind
+
+theorem determinism : Step t t₁ → Step t t₂ → t₁ = t₂ := by
+  intro s1 s2
+  induction s1 generalizing t₂ <;> cases s2
+  all_goals (
+    try contradiction
+    try grind
+  )
+  · rename_i s
+    cases s
+    cases nv_no_step (by assumption) (by assumption)
+  · rename_i s ih
+    cases s
+    cases nv_no_step (by assumption) (by assumption)
+  · rename_i s
+    cases s
+    cases nv_no_step (by assumption) (by assumption)
+  · rename_i s ih
+    cases s
+    cases nv_no_step (by assumption) (by assumption)
+
+def Normal : Term → Prop
+| t => ¬ ∃ t', Step t t'
+
+lemma nv_is_normal : NatV t → Normal t := by
+  intro hnv
+  induction t <;> cases hnv
+              <;> intro ⟨ t', hstep ⟩
+              <;> cases hstep
+  rename_i ih hnv t' s
+  exact ih hnv ⟨ t', s ⟩
+
+theorem value_is_normal : Value v → Normal v := by
+  intro hv
+  cases hv <;> intro ⟨ t', hstep⟩
+  · cases hstep
+  · cases hstep
+  · apply nv_is_normal (by assumption) ⟨ t', hstep ⟩
+
+def Stuck : Term → Prop
+| t => Normal t ∧ ¬ Value t
+
+inductive BigStep : Term → Term → Prop
+| Value : Value v → BigStep v v
+-- Do we need Value v in those two cases below?
+| IfTrue : Value v → BigStep c Term.True → BigStep t v → BigStep (Term.If c t e) v
+| IfFalse : Value v → BigStep c Term.False → BigStep e v → BigStep (Term.If c t e) v
+| Succ : NatV v → BigStep t v → BigStep (Term.Succ t) (Term.Succ v)
+| PredZero : BigStep t Term.Zero → BigStep (Term.Pred t) Term.Zero
+| PredSucc : NatV v → BigStep t (Term.Succ v) → BigStep (Term.Pred t) v
+| IsZeroZero : BigStep t Term.Zero → BigStep (Term.IsZero t) Term.True
+| IsZeroSucc : NatV v → BigStep t (Term.Succ v) → BigStep (Term.IsZero t) Term.False
+
+theorem big_step_is_multi_step : BigStep t v ↔ MultiStep t v := by
+  constructor
+  · sorry
+  · sorry
+
+end Naturals
+
+end Untyped
